feat: add properties to BoundedBacktracker.SearchState

Regex/Backtrack.lean
@@ -55,66 +55,81 @@ instance {α β : Type} [Inhabited β] : Inhabited (ST.Ref β (Array α)) where
 
 end Array.Ref
 
+@[simp] def CharPos.posInRange (s : Substring) (pos : String.Pos) :=
+  s.startPos ≤ pos ∧ pos ≤ s.stopPos
+
 /-- Char position in a substring-/
-structure CharPos where
-  /-- substring -/
-  s : Substring
+structure CharPos (s : Substring) where
   /-- current position -/
   pos : String.Pos := ⟨0⟩
   /-- char at current position -/
   curr? : Option Char := none
   /-- char at previous position -/
   prev? : Option Char := none
+  /-- `pos` is in range of substring `s` -/
+  isPosInRange : CharPos.posInRange s pos
 
-instance : Inhabited CharPos := ⟨default, default, none, none⟩
+abbrev CharPos.PosInRange s := { pos : String.Pos // CharPos.posInRange s pos }
 
-instance : ToString CharPos where
+instance : Inhabited (CharPos default) := ⟨default, none, none, by simp; decide⟩
+
+instance : ToString (CharPos s) where
   toString s := s!"{s.pos} {s.curr?} {s.prev?}"
 
 namespace CharPos
+
+def toSlotEntry («at»: CharPos input) : CharPos.PosInRange input :=
+  ⟨«at».pos, «at».isPosInRange⟩
 
 def get? (s : Substring) («at» : String.Pos) : Option Char :=
   if «at» < s.stopPos then s.get «at» else none
 
 /-- create a CharPos from `s` and position `«at»` -/
-def create (s : Substring) («at» : String.Pos) : CharPos :=
+def create (s : Substring) («at» : String.Pos) (h : s.startPos ≤ «at» ∧ «at» ≤ s.stopPos )
+    : CharPos s :=
   let prev? := if «at» = 0 then none else get? s (s.prev «at»)
-  ⟨s, «at», get? s «at», prev?⟩
+  ⟨«at», get? s «at», prev?, h⟩
 
-def prevOf (offset : Nat) (cp : CharPos) : Option CharPos :=
+def prevOf (offset : Nat) (cp : CharPos s) : Option (CharPos s) :=
   if offset ≤ cp.pos.byteIdx then
-    let pos := cp.s.prevn offset cp.pos
-    some (create cp.s pos)
+    let pos := s.prevn offset cp.pos
+    if h : s.startPos ≤ pos ∧ pos ≤ s.stopPos
+    then some (create s pos h)
+    else none
   else none
 
 /-- to next position CharPos of `cp` -/
-def next (cp : CharPos) : CharPos :=
-  if cp.pos >= cp.s.stopPos then cp
+def next (cp : CharPos s) : CharPos s :=
+  if cp.pos >= s.stopPos then cp
   else
     match cp.curr? with
     | some c =>
       let nextPos : String.Pos := ⟨cp.pos.byteIdx + c.utf8Size⟩
-      {cp with pos := nextPos, prev? := cp.curr?, curr? := get? cp.s nextPos}
+      if h : s.startPos ≤ nextPos ∧ nextPos ≤ s.stopPos
+      then {cp with pos := nextPos, prev? := cp.curr?, curr? := get? s nextPos,
+                    isPosInRange := h}
+      else cp
     | none => cp
 
 /-- is CharPos at start position -/
-def atStart (cp : CharPos) : Bool :=
-  cp.pos = cp.s.startPos
+def atStart (cp : CharPos s) : Bool :=
+  cp.pos = s.startPos
 
 /-- is CharPos at stop position -/
-def atStop (cp : CharPos) : Bool :=
-  cp.pos = cp.s.stopPos
+def atStop (cp : CharPos s) : Bool :=
+  cp.pos = s.stopPos
 
 end CharPos
 
 /-- Represents a stack frame on the heap while doing backtracking. -/
-inductive Frame (n : Nat) where
+inductive Frame (n : Nat) (s : Substring) where
   /-- Look for a match starting at `sid` and the given position in the haystack. -/
-  | Step (sid: Fin n) («at»: CharPos) : Frame n
+  | Step (sid: Fin n) («at»: CharPos s) : Frame n s
   /-- Reset the given `slot` to the given `offset` (which might be `None`). -/
-  | RestoreCapture (role : Capture.Role) (slot: Nat) (offset: Nat × Nat × Option String.Pos) : Frame n
+  | RestoreCapture (role : Capture.Role) (slot: Nat)
+      (offset: Nat × Nat × Option (CharPos.PosInRange s)) : Frame n s
 
-instance : ToString $ Frame n where
+instance : ToString $ Frame n s where
   toString frame :=
     match frame with
     | .Step sid «at» => s!"Step({sid}, {«at».pos})"
@@ -138,46 +153,46 @@ private def compare (a : Fin n × String.Pos) (b : Fin n × String.Pos) : Orderi
   else Ordering.gt
 
 /-- The stack of frames  -/
-abbrev Stack n := List $ Frame n
+abbrev Stack n s := List $ Frame n s
 
 namespace Stack
 
 /-- Push frame to stack  -/
-@[inline] def push (stack : Stack n) (v : Frame n) : Stack n :=
+@[inline] def push (stack : Stack n s) (v : Frame n s) : Stack n s :=
   v :: stack
 
 /-- pop head frame from stack  -/
-@[inline] def pop? (stack : Stack n) : Option (Frame n × Stack n) :=
+@[inline] def pop? (stack : Stack n s) : Option (Frame n s × Stack n s) :=
   match stack with
   | [] => none
   | head :: tail => (head, tail)
 
-theorem pop?_some_lt (s : Stack n) (h : pop? s = some (a, s1)) : s1.length < s.length := by
+theorem pop?_some_lt (s : Stack n s) (h : pop? s = some (a, s1)) : s1.length < s.length := by
   have : s = a :: s1 := by unfold pop? at h; split at h <;> simp_all
   rw [this]
   exact Nat.lt_add_one (List.length s1)
 
 /-- append stacks -/
-@[inline] def append (stack1 stack2 : Stack n) : Stack n :=
+@[inline] def append (stack1 stack2 : Stack n s) : Stack n s :=
   match stack2 with
   | v1 :: v2 :: [] => v2 :: v1 :: stack1
   | _ => List.append (stack2.reverse) stack1
 
-@[inline] def toStack (arr : Array $ Frame n) : Stack n :=
+@[inline] def toStack (arr : Array $ Frame n s) : Stack n s :=
   arr |> Array.toList
 
 end Stack
 
-instance : Inhabited $ Stack 0 := ⟨[]⟩
+instance : Inhabited $ Stack default default := ⟨[]⟩
 
 /-- The encoded set of (Fin n, HaystackOffset) pairs that have been visited
     by the backtracker within a single search. Optimization: encode as bits -/
 abbrev Visited := Array UInt8
 
 /-- State of the backtracking search -/
-@[ext] structure SearchState (n : Nat) where
+@[ext] structure SearchState (n : Nat) (input : Substring) where
   /-- Stack used on the heap for doing backtracking -/
-  stack: Stack n
+  stack: Stack n input
   /-- The encoded set of (Fin n, HaystackOffset) pairs that have been visited
     by the backtracker within a single search. -/
   visited : ST.Ref Nat Visited
@@ -185,12 +200,10 @@ abbrev Visited := Array UInt8
   countVisited : Nat
   /-- current state -/
   sid: Fin n
-  /-- input string -/
-  input : Substring
   /-- position in input string -/
-  «at» : CharPos
-  /-- slots, positions of captures in haystack -/
-  slots: Array (Nat × Nat × (Option String.Pos))
+  «at»: CharPos input
+  /-- slots, positions of captures in `input` -/
+  slots: Array (Nat × Nat × (Option (CharPos.PosInRange input)))
   /-- recent captures of capture groups -/
   recentCaptures: Array (Option (String.Pos × String.Pos))
   /-- is logging enabled -/
@@ -206,7 +219,8 @@ namespace SearchState
 
 /-- create the SearchState from an NFA -/
 def fromNfa (nfa : Checked.NFA) (input : Substring) («at» : String.Pos) (logEnabled : Bool)
-    (h : 0 < nfa.n) : SearchState nfa.n :=
+  (h : 0 < nfa.n ∧ input.startPos ≤ «at» ∧ «at» ≤ input.stopPos )
+    : SearchState nfa.n input :=
   let slotIdxs : Array (Nat × Nat) :=
     nfa.states
     |> Array.filterMap (fun s =>
@@ -214,7 +228,7 @@ def fromNfa (nfa : Checked.NFA) (input : Substring) («at» : String.Pos) (logEn
         | Checked.State.Capture _ _ _ g s => some (s, g)
         | _ => none)
   let sorted := Array.qsort slotIdxs (fun (a, _) (b, _) => a < b) |> Array.unique
-  let slots : Array (Nat × Nat × (Option String.Pos)) :=
+  let slots : Array (Nat × Nat × (Option (CharPos.PosInRange input))) :=
     sorted |> Array.map (fun (s, g) => (s, g, none))
 
   let recentCaptures : Array $ Option (String.Pos × String.Pos) :=
@@ -225,9 +239,8 @@ def fromNfa (nfa : Checked.NFA) (input : Substring) («at» : String.Pos) (logEn
     visited := Array.Ref.mkRef <|
       Array.mkArray ((nfa.states.size + 1) * (input.stopPos.byteIdx - input.startPos.byteIdx +1)) 0
     countVisited := 0
-    sid := ⟨0, h⟩
-    input := input
-    «at» := CharPos.create input «at»
+    sid := ⟨0, h.left⟩
+    «at» := CharPos.create input «at» h.right
     slots := slots
     recentCaptures := recentCaptures
     logEnabled := logEnabled
@@ -242,9 +255,85 @@ instance : Nonempty Visited := ⟨#[]⟩
 
 namespace Visited
 
-/-- get encoded index of Fin n an CharPos in visited array -/
-def index (sid : Fin n) (cp : CharPos) : Nat :=
-  (sid + 1) * (cp.s.stopPos.byteIdx - cp.s.startPos.byteIdx + 1) + cp.pos.byteIdx
+/-- get encoded index of Fin n and CharPos in visited array -/
+def index (sid : Fin n) (cp : CharPos s) : Nat :=
+  sid * (s.stopPos.byteIdx - s.startPos.byteIdx + 1)
+  + cp.pos.byteIdx - s.startPos.byteIdx
+
+theorem eq_of_linear_eq {a1 b1 a2 b2 x : Nat} (hb1 : b1 < x) (hb2 : b2 < x)
+  (h : a1 * x + b1 = a2 * x + b2) : a1 = a2 ∧ b1 = b2 := by
+  if ha : a1 < a2
+  then
+    have ⟨k, hk⟩ : ∃ k, 0 < k ∧ a1 + k = a2 := by
+      have ⟨k', hk⟩ := Nat.exists_eq_add_of_lt ha
+      exact ⟨k' + 1, by omega⟩
+    rw [← hk.right] at h
+    have : a1 * x + b1 = a1 * x + k * x + b2 := by
+      have := Nat.mul_add x a1 k
+      rw [Nat.mul_comm] at this
+      rw [this] at h
+      rw [@Nat.mul_comm x a1, @Nat.mul_comm x k] at h
+      exact h
+    have : b1 = k * x + b2 := by omega
+    have : ¬ b1 < x := by
+      have : k * x ≤ b1 := by omega
+      have : x ≤ k * x := by exact Nat.le_mul_of_pos_left x hk.left
+      omega
+    contradiction
+  else if ha : a2 < a1
+  then
+    have ⟨k, hk⟩ : ∃ k, 0 < k ∧ a2 + k = a1 := by
+      have ⟨k', hk⟩ := Nat.exists_eq_add_of_lt ha
+      exact ⟨k' + 1, by omega⟩
+    rw [← hk.right] at h
+    have : a2 * x + k * x + b1 = a2 * x + b2 := by
+      have := Nat.mul_add x a2 k
+      rw [Nat.mul_comm] at this
+      rw [this] at h
+      rw [@Nat.mul_comm x a2, @Nat.mul_comm x k] at h
+      exact h
+    have : k * x + b1 = b2 := by omega
+    have : ¬ b2 < x := by
+      have : k * x ≤ b2 := by omega
+      have : x ≤ k * x := by exact Nat.le_mul_of_pos_left x hk.left
+      omega
+    contradiction
+  else
+    have : a1 = a2 := by omega
+    rw [this] at h
+    omega
+
+/-- `index` is injective. -/
+theorem index_injective (sid1 sid2 : Fin n) (cp1 cp2 : CharPos s)
+  (heq : index sid1 cp1 = index sid2 cp2)
+    : sid1.val = sid2.val ∧ cp1.pos.byteIdx = cp2.pos.byteIdx := by
+  unfold index at heq
+
+  have hp1 := cp1.isPosInRange
+  have hp2 := cp2.isPosInRange
+  have : s.startPos.byteIdx ≤ s.stopPos.byteIdx := Nat.le_trans hp1.left hp1.right
+  have : s.startPos.byteIdx ≤ s.stopPos.byteIdx := Nat.le_trans hp2.left hp2.right
+  have : s.startPos.byteIdx ≤ cp1.pos.byteIdx := hp1.left
+  have : s.startPos.byteIdx ≤ cp2.pos.byteIdx := hp2.left
+  generalize hx : (s.stopPos.byteIdx - s.startPos.byteIdx + 1) = x at heq
+  have hlt1 : cp1.pos.byteIdx - s.startPos.byteIdx < x := by
+    simp [← hx]
+    suffices cp1.pos.byteIdx - s.startPos.byteIdx
+             ≤ s.stopPos.byteIdx - s.startPos.byteIdx by
+      simp [Nat.lt_add_one_of_le this]
+    exact Nat.sub_le_sub_right hp1.right s.startPos.byteIdx
+  have hlt2 : cp2.pos.byteIdx - s.startPos.byteIdx < x := by
+    simp [← hx]
+    suffices cp2.pos.byteIdx - s.startPos.byteIdx
+             ≤ s.stopPos.byteIdx - s.startPos.byteIdx by
+      simp [Nat.lt_add_one_of_le this]
+    exact Nat.sub_le_sub_right hp2.right s.startPos.byteIdx
+  have h : sid1.val * x + (cp1.pos.byteIdx - s.startPos.byteIdx)
+           = sid2.val * x + (cp2.pos.byteIdx - s.startPos.byteIdx) := by omega
+  have := @eq_of_linear_eq sid1.val (cp1.pos.byteIdx - s.startPos.byteIdx)
+            sid2.val (cp2.pos.byteIdx - s.startPos.byteIdx) x
+            hlt1 hlt2 h
+  omega
 
 private def getRefValue (ref : ST.Ref Nat Visited) : Visited :=
   Array.Ref.getRefValue ref
@@ -255,7 +344,7 @@ private def modifyRefValue (ref : ST.Ref Nat Visited) (index : Nat) (value : UIn
 
 /-- Check if current Fin n and CharPos in SearchState is already visited.
     If not visited mark pair as visited. -/
-def checkVisited (state : SearchState n) : Bool × SearchState n :=
+def checkVisited (state : SearchState n s) : Bool × SearchState n s :=
   let visited := Visited.getRefValue state.visited
   let index := Visited.index state.sid state.at
   if h : index < visited.size then
@@ -266,12 +355,12 @@ def checkVisited (state : SearchState n) : Bool × SearchState n :=
 
 /-- Check if current Fin n and CharPos in SearchState is already visited.
     If not visited mark pair as visited. -/
-def checkVisited' (state : SearchState n) : Bool × SearchState n :=
+def checkVisited' (state : SearchState n s) : Bool × SearchState n s :=
   let (f, s) := checkVisited state
   if f then (true, state)
   else (false, {s with countVisited := state.countVisited + 1})
 
-theorem checkVisited'_false_lt (s : SearchState n) (h : checkVisited' s = (false, s1))
+theorem checkVisited'_false_lt (s : SearchState n input) (h : checkVisited' s = (false, s1))
     : s.countVisited < s1.countVisited := by
   unfold checkVisited' at h
   split at h
@@ -281,7 +370,7 @@ theorem checkVisited'_false_lt (s : SearchState n) (h : checkVisited' s = (false
     simp_all
   simp [Nat.lt_of_succ_le hx]
 
-theorem checkVisited'_true_eq (s : SearchState n) (h : checkVisited' s = (true, s1))
+theorem checkVisited'_true_eq (s : SearchState n input) (h : checkVisited' s = (true, s1))
     : s.countVisited = s1.countVisited ∧ s.stack.length = s1.stack.length := by
   unfold checkVisited' at h
   split at h
@@ -290,27 +379,28 @@ theorem checkVisited'_true_eq (s : SearchState n) (h : checkVisited' s = (true, 
 end Visited
 
 /-- build pairs of subsequent slots -/
-private def toPairs (slots : Array (Nat × Nat × Option String.Pos))
-    : Array (Option (String.Pos × String.Pos)) :=
+private def toPairs (slots : Array (Nat × Nat × Option (CharPos.PosInRange s)))
+    : Array (Option ((CharPos.PosInRange s) × (CharPos.PosInRange s))) :=
   if slots.size % 2 = 0
   then
-    let arr : Array (Option (String.Pos × String.Pos)) := slots.foldl (init := #[])
-      fun acc (i, _) =>
-        if i % 2 = 0 then acc
-        else
-          match slots.get? (i - 1), slots.get? (i) with
-          | some (_, _, some v0), some (_, _, some v1) => acc.push (some (v0,v1))
-          | some (_, _, none), some (_, _, none) => acc.push none
-          | _, _ => acc
+    let arr : Array (Option ((CharPos.PosInRange s) × (CharPos.PosInRange s))) :=
+        slots.foldl (init := #[])
+          fun acc (i, _) =>
+            if i % 2 = 0 then acc
+            else
+              match slots.get? (i - 1), slots.get? (i) with
+              | some (_, _, some v0), some (_, _, some v1) => acc.push (some (v0,v1))
+              | some (_, _, none), some (_, _, none) => acc.push none
+              | _, _ => acc
     arr
   else #[]
 
 /-- add a msg to the SearchState while doing backtracking.  -/
-@[inline] private def withMsg (msg : Unit -> String) (state : SearchState n) : SearchState n :=
+@[inline] private def withMsg (msg : Unit -> String) (state : SearchState n s) : SearchState n s :=
   if state.logEnabled then { state with msgs := state.msgs.push s!"{msg ()}"}
   else state
 
-theorem withMsg_eq {nfa : Checked.NFA} {s s1 : SearchState nfa.n} {msg : Unit -> String}
+theorem withMsg_eq {nfa : Checked.NFA} {s s1 : SearchState nfa.n input} {msg : Unit -> String}
   (h : withMsg  msg s = s1) : s.countVisited = s1.countVisited ∧ s.stack = s1.stack := by
   unfold withMsg at h
   split at h <;> try simp_all
@@ -323,7 +413,7 @@ private def encodeChar? (c: Option Char) : String :=
   | none => "none"
 
 /-- Returns true when [`Look::WordUnicode`] is satisfied `at` the given position in `haystack`. -/
-@[inline] private def is_word_unicode (state : SearchState n) : Bool :=
+@[inline] private def is_word_unicode (state : SearchState n s) : Bool :=
   let word_before :=
     if state.at.atStart then false
     else state.at.prev?.any Unicode.is_word_char
@@ -334,7 +424,7 @@ private def encodeChar? (c: Option Char) : String :=
 
 /-- Returns true when [`Look::WordUnicodeNegate`] is satisfied `at` the
     given position in `haystack`. -/
-@[inline] private def is_word_unicode_negate (state : SearchState n) : Bool :=
+@[inline] private def is_word_unicode_negate (state : SearchState n s) : Bool :=
   let word_before :=
     if state.at.atStart then false
     else state.at.prev?.any Unicode.is_word_char
@@ -345,7 +435,7 @@ private def encodeChar? (c: Option Char) : String :=
 
 /-- Returns true when [`Look::WordStartUnicode`] is satisfied `at` the given position
     in `haystack`. -/
-@[inline] private def is_word_start_unicode (state : SearchState n) : Bool :=
+@[inline] private def is_word_start_unicode (state : SearchState n s) : Bool :=
   let word_before :=
     if state.at.atStart then false
     else state.at.prev?.any Unicode.is_word_char
@@ -356,7 +446,7 @@ private def encodeChar? (c: Option Char) : String :=
 
 /-- Returns true when [`Look::WordEndUnicode`] is satisfied `at` the given position
     in `haystack`. -/
-@[inline] private def is_word_end_unicode (state : SearchState n) : Bool :=
+@[inline] private def is_word_end_unicode (state : SearchState n s) : Bool :=
   let word_before :=
     if state.at.atStart then false
     else state.at.prev?.any Unicode.is_word_char
@@ -367,7 +457,7 @@ private def encodeChar? (c: Option Char) : String :=
 
 /-- Returns true when [`Look::WordStartHalfUnicode`] is satisfied `at` the given position
     in `haystack`. -/
-@[inline] private def is_word_start_half_unicode (state : SearchState n) : Bool :=
+@[inline] private def is_word_start_half_unicode (state : SearchState n s) : Bool :=
   let word_before :=
     if state.at.atStart then false
     else state.at.prev?.any Unicode.is_word_char
@@ -375,17 +465,17 @@ private def encodeChar? (c: Option Char) : String :=
 
 /-- Returns true when [`Look::WordEndHalfUnicode`] is satisfied `at` the given position
     in `haystack`. -/
-@[inline] private def is_word_end_half_unicode (state : SearchState n) : Bool :=
+@[inline] private def is_word_end_half_unicode (state : SearchState n s) : Bool :=
   let word_after :=
     if state.at.atStop then false
     else state.at.curr?.any Unicode.is_word_char
   !word_after
 
-@[inline] private def step_empty (next : Fin n) (state : SearchState n) : SearchState n :=
+@[inline] private def step_empty (next : Fin n) (state : SearchState n s) : SearchState n s :=
   withMsg (fun _ => s!"{state.sid}: Empty -> {next}") {state with sid := next}
 
-@[inline] private def step_next_char (offset : Nat) (next : Fin n) (state : SearchState n)
-    : SearchState n :=
+@[inline] private def step_next_char (offset : Nat) (next : Fin n) (state : SearchState n s)
+    : SearchState n s :=
   match state.at.prevOf offset with
   | some pos =>
     withMsg (fun _ => s!"{state.sid}: NextChar offset {offset} to charpos {pos} -> {next}")
@@ -393,11 +483,11 @@ private def encodeChar? (c: Option Char) : String :=
   | none =>
     withMsg (fun _ => s!"{state.sid}: NextChar offset {offset} failed at charpos {state.at}") state
 
-@[inline] private def step_fail (state : SearchState n) : SearchState n :=
+@[inline] private def step_fail (state : SearchState n s) : SearchState n s :=
   withMsg (fun _ => s!"{state.sid}: Fail") state
 
 /-- eat frames until State `sid` found -/
-@[inline] private def step_eat_until (sid next : Fin n) (state : SearchState n) : SearchState n :=
+@[inline] private def step_eat_until (sid next : Fin n) (state : SearchState n s) : SearchState n s :=
   let stack :=
     state.stack
     |> List.dropWhile (fun s => match s with | .Step f' _ => sid != f' | _ => true)
@@ -410,7 +500,7 @@ private def encodeChar? (c: Option Char) : String :=
     withMsg (fun _ => s!"{state.sid}: EatUntil failed ") state
 
 /-- eat frames inclusive last occurunce of State `sid`  -/
-@[inline] private def step_eat_to_last (sid next : Fin n) (state : SearchState n) : SearchState n :=
+@[inline] private def step_eat_to_last (sid next : Fin n) (state : SearchState n s) : SearchState n s :=
   let index := state.stack
     |> List.reverse
     |> List.findIdx (fun s => match s with | .Step f' _ => sid = f' | _ => false)
@@ -425,17 +515,17 @@ private def encodeChar? (c: Option Char) : String :=
                          {state with sid := next }
     --withMsg (fun _ => s!"{state.sid}: EatToLast failed ") state
 
-@[inline] private def step_eat (mode : Checked.EatMode n) (next : Fin n) (state : SearchState n)
-    : SearchState n :=
+@[inline] private def step_eat (mode : Checked.EatMode n) (next : Fin n) (state : SearchState n s)
+    : SearchState n s :=
   match mode with
   | .Until sid => step_eat_until sid next state
   | .ToLast sid => step_eat_to_last sid next state
 
-@[inline] private def step_change_frame_step (f t : Fin n) (state : SearchState n) : SearchState n :=
-  let cond := (fun (s : Frame n) => match s with | .Step f' _ => f != f' | _ => true)
+@[inline] private def step_change_frame_step (f t : Fin n) (state : SearchState n s) : SearchState n s :=
+  let cond := (fun (s : Frame n s) => match s with | .Step f' _ => f != f' | _ => true)
   let stackBeforeSid := state.stack |> List.takeWhile cond
 
-  let slots : Array (Nat × Nat × (Option String.Pos)) :=
+  let slots : Array (Nat × Nat × (Option (CharPos.PosInRange s))) :=
     stackBeforeSid |> List.foldl (fun slots frame =>
         match frame with
         | .RestoreCapture _ slot v =>
@@ -451,11 +541,11 @@ private def encodeChar? (c: Option Char) : String :=
   | _ =>
     withMsg (fun _ => s!"{state.sid}: ChangeFrameStep failed ") state
 
-@[inline] private def step_remove_frame_step (sid : Fin n) (state : SearchState n) : SearchState n :=
-  let cond := (fun (s : Frame n) => match s with | .Step f' _ => sid != f' | _ => true)
+@[inline] private def step_remove_frame_step (sid : Fin n) (state : SearchState n s) : SearchState n s :=
+  let cond := (fun (s : Frame n s) => match s with | .Step f' _ => sid != f' | _ => true)
   let stackBeforeSid := state.stack |> List.takeWhile cond
 
-  let slots : Array (Nat × Nat × (Option String.Pos)) :=
+  let slots : Array (Nat × Nat × (Option { pos // CharPos.posInRange s pos })) :=
     stackBeforeSid |> List.foldl (fun slots frame =>
         match frame with
         | .RestoreCapture _ slot v =>
@@ -472,7 +562,7 @@ private def encodeChar? (c: Option Char) : String :=
     withMsg (fun _ => s!"{state.sid}: RemoveFrameStep failed ") state
 
 @[inline] private def step_look (look : Look) (next : Fin n)
-     (state : SearchState n) : SearchState n :=
+     (state : SearchState n s) : SearchState n s :=
   match look with
   | .Start =>
     if state.at.atStart then
@@ -566,18 +656,18 @@ private def encodeChar? (c: Option Char) : String :=
         (fun _ => s!"PreviousMatch failed at pos {state.at.pos}") state)
   | .ClearMatches =>
     if h : 0 < state.slots.size then
-      let frame : Frame n := Frame.RestoreCapture Capture.Role.Start 0 (state.slots.get 0 h)
+      let frame : Frame n s := Frame.RestoreCapture Capture.Role.Start 0 (state.slots.get 0 h)
       let stack := Stack.push state.stack frame
       let slots := state.slots |> Array.map (fun (s, g, _) =>
-                    if s = 0 then (s, g, state.at.pos) else (s, g, none))
+                    if s = 0 then (s, g, CharPos.toSlotEntry state.at) else (s, g, none))
       (withMsg (fun _ => s!"{state.sid}: Look.ClearMatches stack {stack} slots {slots} -> {next}")
                           {state with stack := stack, slots := slots, sid := next})
     else
       (withMsg
         (fun _ => s!"ClearMatches failed at pos {state.at.pos}, no slots") state)
 
-@[inline] private def step_byterange (trans : Checked.Transition n) (state : SearchState n)
-    : SearchState n :=
+@[inline] private def step_byterange (trans : Checked.Transition n) (state : SearchState n s)
+    : SearchState n s :=
   if state.at.atStop then
     (withMsg (fun _ =>
       s!"{state.sid}: ByteRange failed at stop")
@@ -594,8 +684,8 @@ private def encodeChar? (c: Option Char) : String :=
             s!"{state.sid}: ByteRange failed match '{t}' at charpos {state.at}")
       state)
 
-@[inline] private def step_backreference_loop (s : String) (i : Nat) (case_insensitive : Bool) (cp : CharPos)
-    : Option CharPos :=
+@[inline] private def step_backreference_loop (s : String) (i : Nat) (case_insensitive : Bool)
+  (cp : CharPos input) : Option (CharPos input) :=
   if i < s.length
   then
     if cp.atStop then none else
@@ -611,16 +701,16 @@ private def encodeChar? (c: Option Char) : String :=
     else none
   else some cp
 
-@[inline] private def step_backreference (b : Nat) (case_insensitive : Bool) (next : Fin n) (state : SearchState n)
-    : SearchState n :=
+@[inline] private def step_backreference (b : Nat) (case_insensitive : Bool) (next : Fin n)
+  (state : SearchState n s) : SearchState n s :=
   if h : b < state.recentCaptures.size then
     match state.recentCaptures.get b h with
     | some (f, t) =>
-        let s := state.input.extract f t |>.toString
-        match step_backreference_loop s 0 case_insensitive state.at with
+        let s' := s.extract f t |>.toString
+        match step_backreference_loop s' 0 case_insensitive state.«at» with
         | some cp =>
-            (withMsg (fun _ => s!"{state.sid}: Backreference {b} '{s}' matched from charpos {state.at} to {cp} -> {next}")
-                {state with sid := next, «at» := cp})
+            (withMsg (fun _ => s!"{state.sid}: Backreference {b} '{s'}' matched from charpos {state.at} to {cp} -> {next}")
+                {state with sid := next, «at» := cp })
         | none =>
           (withMsg (fun _ =>
             s!"{state.sid}: Backreference '{b}' failed at charpos {state.at}, no match with '{s}'")
@@ -635,7 +725,7 @@ private def encodeChar? (c: Option Char) : String :=
     state)
 
 @[inline] private def step_sparse_transitions (_ : Checked.NFA)
-    (transitions : Array $ Checked.Transition n)  (state : SearchState n) : SearchState n :=
+    (transitions : Array $ Checked.Transition n)  (state : SearchState n s) : SearchState n s :=
   if state.at.atStop then
       (withMsg
         (fun _ =>
@@ -652,7 +742,7 @@ private def encodeChar? (c: Option Char) : String :=
         (fun _ =>
             s!"{state.sid}: SparseTransitions failed  at charpos {state.at}") state)
 
-@[inline] private def step_union (alts : Array $ Fin n) (state : SearchState n) : SearchState n :=
+@[inline] private def step_union (alts : Array $ Fin n) (state : SearchState n s) : SearchState n s :=
   match alts with
   | #[alt1, alt2] =>
     let stack := Stack.push state.stack (Frame.Step alt2 state.at)
@@ -668,8 +758,8 @@ private def encodeChar? (c: Option Char) : String :=
         {state with sid := alt, stack := stack})
     | none => state
 
-@[inline] private def step_union_reverse (alts : Array $ Fin n) (state : SearchState n)
-    : SearchState n :=
+@[inline] private def step_union_reverse (alts : Array $ Fin n) (state : SearchState n s)
+    : SearchState n s :=
   match alts with
   | #[alt1, alt2] =>
     let stack := Stack.push state.stack (Frame.Step alt1 state.at)
@@ -686,16 +776,16 @@ private def encodeChar? (c: Option Char) : String :=
     | none => state
 
 @[inline] private def step_binary_union (alt1 alt2 : Fin n)
-     (state : SearchState n) : SearchState n :=
+     (state : SearchState n s) : SearchState n s :=
   (withMsg (fun _ => s!"BinaryUnion {state.sid} -> {alt1}")
        {state with sid := alt1, stack := Stack.push state.stack (Frame.Step alt2 state.at)})
 
 @[inline] private def step_change_capture_slot (next : Fin n) (slot : Nat)
-     (state : SearchState n) : SearchState n :=
+     (state : SearchState n s) : SearchState n s :=
   if h : slot < state.slots.size
   then
     let (s, g, _) := state.slots.get slot h
-    let slots := state.slots.set slot (s, g, some state.at.pos) h
+    let slots := state.slots.set slot (s, g, CharPos.toSlotEntry state.at) h
     (withMsg (fun _ => s!"{state.sid}: ChangeCaptureSlot slot {slot} slots {slots} -> {next}")
                 {state with sid := next, slots := slots })
   else
@@ -703,13 +793,13 @@ private def encodeChar? (c: Option Char) : String :=
                 state)
 
 @[inline] private def step_capture (role : Capture.Role)(next : Fin n) (group slot : Nat)
-     (state : SearchState n) : SearchState n :=
+     (state : SearchState n s) : SearchState n s :=
   let (stack, slots, recentCaptures) :=
     if h : slot < state.slots.size
     then
       let (s, g, _) := state.slots.get slot h
       let frame := Frame.RestoreCapture role slot (state.slots.get slot h)
-      let slots := state.slots.set slot (s, g, state.at.pos) h
+      let slots := state.slots.set slot (s, g, CharPos.toSlotEntry state.at) h
       let recentCaptures :=
         if role == Capture.Role.End then
 
@@ -729,13 +819,13 @@ private def encodeChar? (c: Option Char) : String :=
                 {state with sid := next, slots := slots, stack := stack, recentCaptures := recentCaptures })
 
 @[inline] private def step_match (pattern_id : PatternID)
-     (state : SearchState n) : SearchState n :=
+     (state : SearchState n s) : SearchState n s :=
   (withMsg (fun _ => s!"Match {state.sid}")
           {state with halfMatch := some ⟨pattern_id, state.at.pos⟩})
 
 /-- execute next step in NFA if state not already visited -/
 @[inline] private def toNextStep (nfa : Checked.NFA) (state : Checked.State n)
-    (searchState : SearchState n) : SearchState n :=
+    (searchState : SearchState n s) : SearchState n s :=
   match state with
   | .Empty next => step_empty next searchState
   | .NextChar offset next => step_next_char offset next searchState
@@ -754,12 +844,12 @@ private def encodeChar? (c: Option Char) : String :=
   | .Match pattern_id => step_match pattern_id searchState
 
 @[inline] private def toNextStep' (nfa : Checked.NFA) (state : Checked.State nfa.n)
-    (searchState : SearchState nfa.n) : SearchState nfa.n :=
+    (searchState : SearchState nfa.n s) : SearchState nfa.n s :=
   let searchState' := toNextStep nfa  state searchState
   -- countVisited is not changed in `toNextStep`
   {searchState' with countVisited := searchState.countVisited}
 
-theorem toNextStep'_eq {nfa : Checked.NFA} {state : Checked.State nfa.n} {s s1 : SearchState nfa.n}
+theorem toNextStep'_eq {nfa : Checked.NFA} {state : Checked.State nfa.n} {s s1 : SearchState nfa.n input}
   {msg : Unit → String}
   (h : toNextStep' nfa state (withMsg msg s) = s1) : s.countVisited = s1.countVisited := by
   unfold toNextStep' at h
@@ -768,8 +858,8 @@ theorem toNextStep'_eq {nfa : Checked.NFA} {state : Checked.State nfa.n} {s s1 :
   split at h <;> try simp_all
 
 /-- execute next step in NFA if state not already visited. Returns true if steps available. -/
-@[inline] private def toNextStepChecked (nfa : Checked.NFA) (state : SearchState nfa.n)
-    : Bool × SearchState nfa.n :=
+@[inline] private def toNextStepChecked (nfa : Checked.NFA) (state : SearchState nfa.n s)
+    : Bool × SearchState nfa.n s :=
   match Visited.checkVisited' state with
   | (false, state') =>
       let state := nfa.states.get state'.sid.val (by
@@ -782,7 +872,7 @@ theorem toNextStep'_eq {nfa : Checked.NFA} {state : Checked.State nfa.n} {s s1 :
                 --state')
   | _ => (false, (withMsg (fun _ => s!"{state.sid}: isVisited charpos {state.at}") state))
 
-theorem toNextStepChecked_true_lt (nfa : Checked.NFA) (s s1 : SearchState nfa.n)
+theorem toNextStepChecked_true_lt (nfa : Checked.NFA) (s s1 : SearchState nfa.n input)
   (h : toNextStepChecked nfa s = (true, s1)) : s.countVisited < s1.countVisited := by
   unfold toNextStepChecked at h
   split at h <;> simp_all
@@ -793,26 +883,26 @@ theorem toNextStepChecked_true_lt (nfa : Checked.NFA) (s s1 : SearchState nfa.n)
     simp [Visited.checkVisited'_false_lt s hcv]
   exact Nat.lt_of_lt_of_eq hlt (id (Eq.symm heq))
 
-theorem toNextStepChecked_false_eq (nfa : Checked.NFA) (s s1 : SearchState nfa.n)
+theorem toNextStepChecked_false_eq (nfa : Checked.NFA) (s s1 : SearchState nfa.n input)
   (h : toNextStepChecked nfa s = (false, s1))
     : s.countVisited = s1.countVisited ∧ s.stack = s1.stack := by
   unfold toNextStepChecked at h
   split at h <;> try simp_all
   simp [withMsg_eq h]
 
-@[inline] private def visitedSize (state : SearchState n) : Nat :=
+@[inline] private def visitedSize (state : SearchState n s) : Nat :=
    (Visited.getRefValue state.visited).size
 
-@[inline] private def unvisited (state : SearchState n) : Nat :=
+@[inline] private def unvisited (state : SearchState n s) : Nat :=
    (visitedSize state) - state.countVisited
 
 /-- execute next steps in NFA. -/
-def steps (nfa : Checked.NFA) (state : SearchState nfa.n) : SearchState nfa.n :=
+def steps (nfa : Checked.NFA) (state : SearchState nfa.n s) : SearchState nfa.n s :=
   match toNextStepChecked nfa state with
   | (true, state) => loop nfa state
   | (false, state) => state
 where
-  loop (nfa : Checked.NFA) (state : SearchState nfa.n) : SearchState nfa.n :=
+  loop (nfa : Checked.NFA) (state : SearchState nfa.n s) : SearchState nfa.n s :=
     match h : toNextStepChecked nfa state with
     | (true, state') =>
       have h2 : state.countVisited < state'.countVisited :=
@@ -828,7 +918,7 @@ where
     | (false, state) => state
 termination_by unvisited state
 
-theorem steps_loop_le (nfa : Checked.NFA) (s s1 : SearchState nfa.n) (h : steps.loop nfa s = s1)
+theorem steps_loop_le (nfa : Checked.NFA) (s s1 : SearchState nfa.n input) (h : steps.loop nfa s = s1)
     : s.countVisited ≤ s1.countVisited := by
   unfold steps.loop at h
   split at h <;> try simp_all
@@ -851,7 +941,7 @@ theorem steps_loop_le (nfa : Checked.NFA) (s s1 : SearchState nfa.n) (h : steps.
     simp [Nat.le_of_eq h2.left]
 termination_by unvisited s
 
-theorem steps_lt_or_eq_lt (nfa : Checked.NFA) (s s1 : SearchState nfa.n) (h : steps nfa s = s1)
+theorem steps_lt_or_eq_lt (nfa : Checked.NFA) (s s1 : SearchState nfa.n input) (h : steps nfa s = s1)
   : s.countVisited < s1.countVisited
     ∨ s.countVisited = s1.countVisited ∧ s.stack.length = s1.stack.length := by
   unfold steps at h
@@ -865,8 +955,8 @@ theorem steps_lt_or_eq_lt (nfa : Checked.NFA) (s s1 : SearchState nfa.n) (h : st
       toNextStepChecked_false_eq nfa s s1 heq
     simp_all
 
-@[inline] private def toNextFrameStep (nfa : Checked.NFA) (state : SearchState nfa.n)
-    : Bool × SearchState nfa.n :=
+@[inline] private def toNextFrameStep (nfa : Checked.NFA) (state : SearchState nfa.n s)
+    : Bool × SearchState nfa.n s :=
   let state' := steps nfa state
   match state'.halfMatch with
   | some _ => (false, state')
@@ -877,7 +967,7 @@ theorem steps_lt_or_eq_lt (nfa : Checked.NFA) (s s1 : SearchState nfa.n) (h : st
                     then state'.msgs.push s!"{state'.sid}: Backtrack.Loop stack {state'.stack}"
                     else state'.msgs})
 
-theorem toNextFrameStep_true_lt_or_eq_lt (nfa : Checked.NFA) (s s1 : SearchState nfa.n)
+theorem toNextFrameStep_true_lt_or_eq_lt (nfa : Checked.NFA) (s s1 : SearchState nfa.n input)
   (h : toNextFrameStep nfa s = (true, s1)) :
     s.countVisited < s1.countVisited ∨ s.countVisited = s1.countVisited
         ∧ s.stack.length = s1.stack.length := by
@@ -895,8 +985,9 @@ theorem toNextFrameStep_true_lt_or_eq_lt (nfa : Checked.NFA) (s s1 : SearchState
   have : state'.stack.length = s1.stack.length := by simp_all
   omega
 
-@[inline] private def toNextFrameRestoreCapture (slot : Nat) (offset : Nat × Nat × Option String.Pos)
-  (stack : Stack n) (state : SearchState n) : Bool × SearchState n :=
+@[inline] private def toNextFrameRestoreCapture (slot : Nat)
+  (offset : Nat × Nat × Option (CharPos.PosInRange s))
+  (stack : Stack n s) (state : SearchState n s) : Bool × SearchState n s :=
   if h : slot < state.slots.size
   then
     let state := {state with slots := state.slots.set slot offset h, stack := stack}
@@ -904,8 +995,9 @@ theorem toNextFrameStep_true_lt_or_eq_lt (nfa : Checked.NFA) (s s1 : SearchState
     (true, state)
   else (false, state)
 
-theorem toNextFrameRestoreCapture_true_lt_or_eq_lt (slot : Nat) (offset : Nat × Nat × Option String.Pos)
-  (stack : Stack n) (s : SearchState n)
+theorem toNextFrameRestoreCapture_true_lt_or_eq_lt (slot : Nat)
+  (offset : Nat × Nat × Option (CharPos.PosInRange s))
+  (stack : Stack n s) (s : SearchState n s)
     (h : toNextFrameRestoreCapture slot offset stack s = (true, s1))
     : s.countVisited = s1.countVisited ∧ stack = s1.stack := by
   unfold toNextFrameRestoreCapture at h
@@ -915,8 +1007,8 @@ theorem toNextFrameRestoreCapture_true_lt_or_eq_lt (slot : Nat) (offset : Nat ×
 
 /-- execute steps in next frame. Returns false if no more frame available
     or match is found. -/
-@[inline] private def toNextFrame (nfa : Checked.NFA) (state : SearchState nfa.n)
-    : Bool × SearchState nfa.n :=
+@[inline] private def toNextFrame (nfa : Checked.NFA) (state : SearchState nfa.n s)
+    : Bool × SearchState nfa.n s :=
   match Stack.pop? state.stack with
   | some (frame, stack) =>
       match frame with
@@ -930,7 +1022,7 @@ theorem toNextFrameRestoreCapture_true_lt_or_eq_lt (slot : Nat) (offset : Nat ×
   | none =>
     (false, (withMsg (fun _ => s!"{state.sid}: stack empty ") state))
 
-theorem toNextFrame_true_lt (nfa : Checked.NFA) (s s1 : SearchState nfa.n)
+theorem toNextFrame_true_lt (nfa : Checked.NFA) (s s1 : SearchState nfa.n input)
   (h : toNextFrame nfa s = (true, s1))
     : s.countVisited < s1.countVisited
       ∨ s.countVisited = s1.countVisited ∧ s1.stack.length < s.stack.length := by
@@ -938,9 +1030,9 @@ theorem toNextFrame_true_lt (nfa : Checked.NFA) (s s1 : SearchState nfa.n)
   split at h
   split at h <;> try simp
   · rename_i stack _ sid _at heq
-    let state : SearchState nfa.n :=
+    let state : SearchState nfa.n input :=
       { stack := stack, visited := s.visited, countVisited := s.countVisited, sid := sid,
-        input := s.input, «at» := _at,
+        «at» := _at,
         slots := s.slots, logEnabled := s.logEnabled,
         recentCaptures := s.recentCaptures
         msgs := if s.logEnabled
@@ -967,7 +1059,7 @@ theorem toNextFrame_true_lt (nfa : Checked.NFA) (s s1 : SearchState nfa.n)
   · have hx : false = true := by simp_all [h]
     contradiction
 
-theorem searchState_lexLt (nfa : Checked.NFA) (s s1 : SearchState nfa.n)
+theorem searchState_lexLt (nfa : Checked.NFA) (s s1 : SearchState nfa.n input)
   (h1 : s.countVisited < visitedSize s) (h2 : visitedSize s = visitedSize s1)
   (h : toNextFrame nfa s = (true, s1)) : unvisited s1 < unvisited s
             ∨ unvisited s1 = unvisited s ∧ s1.stack.length < s.stack.length := by
@@ -978,7 +1070,7 @@ theorem searchState_lexLt (nfa : Checked.NFA) (s s1 : SearchState nfa.n)
     toNextFrame_true_lt nfa s s1 h
   omega
 
-private def collect_info (state : SearchState n) : Array String :=
+private def collect_info (state : SearchState n s) : Array String :=
   let visited := Visited.getRefValue state.visited
   let values := visited |> Array.filter (· = 1) |>.size
   #[
@@ -988,7 +1080,7 @@ private def collect_info (state : SearchState n) : Array String :=
   ]
 
 /-- BoundedBacktrack search -/
-def backtrack (nfa : Checked.NFA)  (state : SearchState nfa.n) : SearchState nfa.n :=
+def backtrack (nfa : Checked.NFA)  (state : SearchState nfa.n s) : SearchState nfa.n s :=
   let frame := Frame.Step state.sid state.at
   let state := (withMsg (fun _ => s!"Backtrack sid {state.sid} charpos {state.at.pos}")
        {state with stack := Stack.push state.stack frame})
@@ -996,7 +1088,7 @@ def backtrack (nfa : Checked.NFA)  (state : SearchState nfa.n) : SearchState nfa
   -- let state := {state with msgs := state.msgs ++ (collect_info state)}
   state
 where
-  loop (nfa : Checked.NFA) (state : SearchState nfa.n) : SearchState nfa.n :=
+  loop (nfa : Checked.NFA) (state : SearchState nfa.n s) : SearchState nfa.n s :=
     match h : toNextFrame nfa state with
     | (true, state') =>
       -- let state := {state with backtracks := state.backtracks + 1}
@@ -1021,8 +1113,8 @@ private def dropLastWhile (arr : Array  α) (p :  α -> Bool) : Array α :=
 
 /-- Search for the first match of this regex in the haystack. -/
 private def slots' (s : Substring) («at» : String.Pos) (nfa : Checked.NFA) (logEnabled : Bool)
-    : (Array String) × (Array (Option (String.Pos × String.Pos))) :=
-  if h : 0 < nfa.n then
+    : (Array String) × (Array (Option (CharPos.PosInRange s × CharPos.PosInRange s))) :=
+  if h : 0 < nfa.n ∧ s.startPos ≤ «at» ∧ «at» ≤ s.stopPos then
     let state := backtrack nfa (SearchState.fromNfa nfa s «at» logEnabled h)
     let pairs := toPairs state.slots
     (state.msgs, dropLastWhile pairs (·.isNone))
@@ -1032,7 +1124,7 @@ private def slots' (s : Substring) («at» : String.Pos) (nfa : Checked.NFA) (lo
     simulate the unanchored prefix with looping. -/
 private def slotsWithUnanchoredPrefix (s : Substring) («at» : String.Pos) (nfa : Checked.NFA)
   (logEnabled : Bool) (init : Array String)
-    : (Array String) × (Array (Option (String.Pos × String.Pos))) :=
+    : (Array String) × (Array (Option (CharPos.PosInRange s × CharPos.PosInRange s))) :=
   if h: s.stopPos.byteIdx <= «at».byteIdx then
     let (msgs, slots) := slots' s «at» nfa logEnabled
     (init ++ msgs, slots)
@@ -1049,18 +1141,16 @@ private def slotsWithUnanchoredPrefix (s : Substring) («at» : String.Pos) (nfa
     | _ => (init ++ msgs, slots)
 termination_by s.stopPos.byteIdx - «at».byteIdx
 
-private def toMatches (s : Substring) (slots : Array (Option (String.Pos × String.Pos)))
+private def toMatches (s : Substring) (slots : Array (Option (
+                     CharPos.PosInRange s × CharPos.PosInRange s)))
     : Array (Option { m : Substring // m.str = s.str }) :=
   slots
   |> Array.map (fun pair =>
       match pair with
       | some (p0, p1) =>
-          if s.startPos ≤ p0
-          then
-            if p1 ≤ s.stopPos
-            then some ⟨⟨s.str, p0, p1⟩, by simp⟩
-            else none
-          else none
+          have : s.startPos ≤ p0.val := p0.property.left
+          have : p1.val ≤ s.stopPos := p1.property.right
+          some ⟨⟨s.str, p0.val, p1.val⟩, by simp⟩
       | none => none)
 
 /-- Search for the first match of this regex in the haystack given and return log msgs and
